OpenvmFv/Spec/ITYPE/ori.lean
@@ -3,7 +3,7 @@ import OpenvmFv.Spec.rX_bits
 
 namespace PureSpec
 
-  structure AddiInput where
+  structure OriInput where
     -- operands
     r1_val : BitVec 32
     imm : BitVec 12
@@ -11,12 +11,12 @@ namespace PureSpec
     -- registers
     PC : BitVec 32
 
-  structure AddiOutput where
+  structure OriOutput where
     -- registers
     nextPC : BitVec 32
     rd : Option (Finset.Icc 1 31 × BitVec 32)
 
-  def execute_ITYPE_addi_pure (input : AddiInput) : AddiOutput := {
+  def execute_ITYPE_ori_pure (input : OriInput) : OriOutput := {
     nextPC := input.PC + 4#32
     rd := if h: input.rd = 0
       then .none
@@ -25,28 +25,28 @@ namespace PureSpec
           input.rd.val,
           by apply Finset.mem_Icc.mpr; omega
         ⟩,
-        input.r1_val + BitVec.signExtend 32 input.imm
+        input.r1_val ||| BitVec.signExtend 32 input.imm
       )
-    : AddiOutput
+    : OriOutput
   }
 
-  lemma execute_ITYPE_addi_pure_equiv
-    (addi_input : AddiInput)
+  lemma execute_ITYPE_ori_pure_equiv
+    (ori_input : OriInput)
     (r1 rd: regidx)
-    (h_input_r1: read_xreg (regidx_to_fin r1) state = EStateM.Result.ok (addi_input.r1_val) state)
-    (h_input_imm: addi_input.imm = imm)
-    (h_input_rd: addi_input.rd = regidx_to_fin rd)
-    (h_input_pc: state.regs.get? Register.PC = .some addi_input.PC)
+    (h_input_r1: read_xreg (regidx_to_fin r1) state = EStateM.Result.ok (ori_input.r1_val) state)
+    (h_input_imm: ori_input.imm = imm)
+    (h_input_rd: ori_input.rd = regidx_to_fin rd)
+    (h_input_pc: state.regs.get? Register.PC = .some ori_input.PC)
   :
     (
       do
         Sail.writeReg Register.nextPC (Sail.BitVec.addInt (← Sail.readReg Register.PC) 4)
-        LeanRV32D.Functions.execute (instruction.ITYPE (imm, r1, rd, iop.ADDI))
+        LeanRV32D.Functions.execute (instruction.ITYPE (imm, r1, rd, iop.ORI))
     ) state =
-    let addi_output := execute_ITYPE_addi_pure addi_input
+    let ori_output := execute_ITYPE_ori_pure ori_input
     (do
-      Sail.writeReg Register.nextPC addi_output.nextPC
-      match addi_output.rd with
+      Sail.writeReg Register.nextPC ori_output.nextPC
+      match ori_output.rd with
         | .some (rd, rd_val) => write_xreg rd rd_val
         | .none => pure ()
       pure (ExecutionResult.Retire_Success ())
@@ -77,7 +77,7 @@ namespace PureSpec
     rewrite [read_xreg_write_reg_state_nextPC _ h_input_r1]
     simp [EStateM.pure]
 
-    simp [execute_ITYPE_addi_pure]
+    simp [execute_ITYPE_ori_pure]
 
     obtain ⟨rd⟩ := rd
     by_cases h_zero: rd = 0
